Various attempts at solving intro lemmas.

theories/intro.v
@@ -24,62 +24,245 @@ Section intro.
 
   Let host_application := @host_application host_function host_instance.
 
+  (* "reduce" checks (state, store, frame, seq -> state, store, frame, seq)? as Prop  *)
   Let reduce : host_state -> store_record -> frame -> seq administrative_instruction ->
                host_state -> store_record -> frame -> seq administrative_instruction -> Prop
       := @reduce _ _.
 
+  (* https://coq.inria.fr/library/Coq.Relations.Relation_Operators.html#clos_refl_trans
+   * Uses "clos_refl_trans" with a "reduce_tuple"
+   *)
   Let reduce_trans := @reduce_trans host_function host_instance.
   
   Let config_tuple := config_tuple host_instance.
 
 
+  (* For all (s of type T), Q, P:
+   * Hypotheses:
+   *  If there exists an s such that (Q s), then P
+   *  (Q s)
+   * Goal: P
+   * Proof:
+   *  Exists s in H0. Apply H0 in H1. Apply H1.
+   *)
   Lemma test: forall {T: Type} (s: T) Q P ,
       ((exists s, Q s) -> P) -> (Q s) -> P.
   Proof.
+    (* Simpler:
+    intros T s Q P H0 H1.
+    apply H0. exists s. apply H1.
+    *)
     move => T s Q P Himpl HQ.
     apply Himpl; eexists; by apply HQ.
   Qed.
-  
-      
 
+  (* Simpler extra practice lemmas *)
+
+  Lemma tuple_to_trans: forall hs1 s1 f1 es1 hs2 s2 f2 es2,
+    reduce_trans (hs1, s1, f1, es1) (hs2, s2, f2, es2) ->
+    reduce_tuple (hs1, s1, f1, es1) (hs2, s2, f2, es2).
+  Proof.
+    intros.
+  Admitted.
+  Lemma reduce_to_tuple: forall hs1 s1 f1 es1 hs2 s2 f2 es2,
+    reduce_tuple (hs1, s1, f1, es1) (hs2, s2, f2, es2) ->
+    reduce hs1 s1 f1 es1 hs2 s2 f2 es2.
+  Proof.
+    intros.
+    unfold reduce_tuple in H.
+    apply H.
+  Qed.
+
+  Lemma reduce_to_trans: forall hs1 s1 f1 es1 hs2 s2 f2 es2,
+    reduce_trans (hs1, s1, f1, es1) (hs2, s2, f2, es2) ->
+    reduce hs1 s1 f1 es1 hs2 s2 f2 es2.
+  Proof.
+    intros.
+    apply reduce_to_tuple.
+    apply tuple_to_trans.
+    apply H.
+  Qed.
+  Lemma reduce_from_trans: forall hs1 s1 f1 es1 hs2 s2 f2 es2,
+    reduce hs1 s1 f1 es1 hs2 s2 f2 es2 ->
+    reduce_trans (hs1, s1, f1, es1) (hs2, s2, f2, es2).
+  Proof.
+    intros. unfold reduce_trans.
+    apply Relations.Relation_Operators.rt_step.
+    unfold reduce_tuple. apply H.
+  Qed.
   
+  Lemma opsem_reduce_seq0: forall hs1 s1 f1 es1 hs2 s2 f2 es2 hs3 s3 f3 es3,
+      reduce hs1 s1 f1 es1 hs2 s2 f2 es2 ->
+      reduce hs2 s2 f2 es2 hs3 s3 f3 es3 ->
+      reduce hs1 s1 f1 es1 hs3 s3 f3 es3.
+  Proof.
+    intros. rename H into H12. rename H0 into H23.
+    cut (reduce_tuple (hs1, s1, f1, es1) (hs2, s2, f2, es2)). 2: { apply H12. } intros H12'.
+    cut (reduce_tuple (hs2, s2, f2, es2) (hs3, s3, f3, es3)). 2: { apply H23. } intros H23'.
+    cut (reduce_trans (hs1, s1, f1, es1) (hs3, s3, f3, es3)). 2 : {
+      apply Relations.Relation_Operators.rt_trans with (hs2, s2, f2, es2).
+      - apply Relations.Relation_Operators.rt_step. apply H12.
+      - apply Relations.Relation_Operators.rt_step. apply H23.
+    } intros H13''.
+    apply reduce_to_trans. apply H13''.
+  Qed.
+
+  Lemma trans_result: forall hs1 s1 f1 es1 hs2 s2 f2 es2,
+    reduce hs1 s1 f1 es1 hs2 s2 f2 es2 ->
+    exists hs3 s3 f3, reduce hs3 s3 f3 [::] hs3 s3 f3 [::] ->
+    reduce hs1 s1 f1 es1 hs3 s3 f3 [::].
+  Proof.
+    intros. (* (Exists stops this proof)
+    apply reduce_to_trans.
+    apply Relations.Relation_Operators.rt_refl.*)
+  Admitted.
+  Lemma trans_split: forall hs1 s1 f1 es1 hs2 s2 f2 es2 es3,
+    reduce_trans (hs1, s1, f1, (es1 ++ es3)) (hs2, s2, f2, (es2 ++ es3)) ->
+    reduce_trans (hs1, s1, f1, es1) (hs2, s2, f2, es2) ->
+    (exists hs3 s3 f3,
+      reduce_trans (hs2, s2, f2, es2) (hs3, s3, f3, [::]) ->
+      reduce_trans (hs2, s2, f2, (es2 ++ es3)) (hs3, s3, f3, es3)) ->
+    reduce_trans (hs1, s1, f1, (es1 ++ es3)) (hs2, s2, f2, (es2 ++ es3)).
+  Proof. (* Test lemma *) Admitted.
+
+
+  (* Operational Semantics: Reduction with equivalent base instructions + identical instruction
+   * If the base instructions reduce to the same result (i.e. are equivalent),
+   *  Appending identical instructions to both sides will still give the same result.
+   *)
+
+Search (_ ++ nil). (* cats0 *)
+Search AI_trap.
+
   (* Reduction of a sequence of commands.
-     There's no `explicit` rule that allows this to be possible, yet this is certainly an expected behaviour.
- *)
+      There's no `explicit` rule that allows this to be possible
+      yet this is certainly an expected behaviour.
+   *)
   Lemma opsem_reduce_seq1: forall hs1 s1 f1 es1 hs2 s2 f2 es2 es0,
       reduce hs1 s1 f1 es1 hs2 s2 f2 es2 ->
       reduce hs1 s1 f1 (es1 ++ es0) hs2 s2 f2 (es2 ++ es0).
   Proof.
+    intros.
+
+    (* Perhaps try to obtain reduce (x, x0, x1, es0) (x, x0, x1, es0)?
+    apply reduce_to_trans. pose proof H as H0. pose proof H as Ht.
+    apply trans_result in H0. destruct H0. destruct H0. destruct H0.
+    apply reduce_from_trans in Ht.
+    
+    cut (reduce_trans (x, x0, x1, [::]) (x, x0, x1, [::])). 2: {
+      apply Relations.Relation_Operators.rt_refl.
+    } intros Ht_33.
+    apply reduce_to_trans in Ht_33. apply H0 in Ht_33 as Ht_13.
+    apply reduce_from_trans in Ht_33. apply reduce_from_trans in Ht_13.
+    (*cut (reduce_trans (hs2, s2, f2, es2) (x, x0, x1, [::])). 2: {
+      apply Relations.Relation_Operators.rt_trans with (hs1, s1, f1, es1).
+      { admit. (* eq, should be symmetric? *) } { apply Ht_13. }
+    } intros Ht_23.*)
+
+    apply trans_split. 2: { apply Ht. } 2: {
+      exists x. exists x0. exists x1. intros Ht_23'.
+      admit.
+    }*)
+
+  (* False, since no guarantee instructions give same output for all inputs
+    cut (reduce_trans (hs1, s1, f1, es0) (hs2, s2, f2, es0)). 2: {
+      admit. 
+    } intros Ht_es0. *)
+    (* (1,1+0) -> (2,2+0) same as (1,1+0) -> (1',1) -> (2',2) -> (2,2+0) *)
+    (* Relation not symmetric so cannot do this; should it be? *)
+
+  (*induction es0 as [|e es' iHyp].
+    - rewrite cats0. rewrite cats0. apply H.*)
+      (* STUCK:
+       *  Case adds instruction between es# and es' instead of at end.
+       *    Could fix with custom induction?
+       *  Also don't know how to simplify reduction regardless.
+       *    Apply Relations.Relation_Operators.rt_trans
+       *      with (y := [iHyp])
+       *    Or Relations.Relation_Operators.rt_step? [Didn't work]
+       *)
+  (*- inversion iHyp. {} destruct e eqn:eEqn; simpl. *)
   Admitted.
 
-  (* Now note that given Wasm's representation of value stack squashed into the instruction list, adding more constants to the bottom of the value stack should not matter as well. *)
+  (* Helper lemma for opsem_reduce_seq2 (reduce one const) *)
+  Lemma opsem_reduce_seq2': forall hs1 s1 f1 es1 hs2 s2 f2 es2 v,
+    is_const v ->
+    reduce hs1 s1 f1 es1 hs2 s2 f2 es2 ->
+    reduce hs1 s1 f1 (v :: es1) hs2 s2 f2 (v :: es2).
+  Proof.
+    intros.
+    destruct v eqn:vEqn; try ( destruct b eqn:bEqn );
+    simpl in H; try ( discriminate ).
+    
+    (* REDUCED DOWN TO SINGLE CASE (STUCK):
+        reduce hs1 s1 f1 (AI_basic (BI_const v0) :: es1)
+              hs2 s2 f2 (AI_basic (BI_const v0) :: es2)
+    *)
+    admit.
+    (*inversion H0; try (apply r_simple (*contructor*)). {
+       
+    }*)
+(*? cut (reduce_tuple (hs1, s1, f1, (AI_basic (BI_const v0) :: es1)) (hs2, s2, f2, (AI_basic (BI_const v0) :: es2))). *)
+(*? induction es1 as [|h1 t1 iHyp1]; induction es2 as [|h2 t2 iHyp2]. { } *)
+(*? inversion H0; try (apply r_simple). { } *)
+  Admitted.
+
+  (* Operational Semantics: Reduction with equivalent base instructions + constant value stack
+   * Given a list/stack of constants,
+   *  Prepending them to equivalent instruction will give the same result.
+   *)
+
+  (* Now note that given Wasm's representation of value stack squashed into the instruction list,
+      adding more constants to the bottom of the value stack should not matter as well. *)
   Lemma opsem_reduce_seq2: forall hs1 s1 f1 es1 hs2 s2 f2 es2 vs,
       const_list vs ->
       reduce hs1 s1 f1 es1 hs2 s2 f2 es2 ->
       reduce hs1 s1 f1 (vs ++ es1) hs2 s2 f2 (vs ++ es2).
   Proof.
-  Admitted.
+      intros. rename H into Hvs. rename H0 into Hred.
+      induction vs as [|v vs' iHyp]; simpl.
+      - apply Hred.
+      - apply Bool.andb_true_iff in Hvs.
+        destruct Hvs as [Hv Hvs']. apply iHyp in Hvs'.
+        apply opsem_reduce_seq2'; (apply Hv || apply Hvs').
+  (*! Uses admitted opsem_reduce_seq2' !*)
+  Qed.
 
-  (* This lemma can of course be derived from the two above. However, its proof itself is
-     even simpler. *)
+
+  (* Operational Semantics: Reduction with equivalent base instructions (combination of above)
+   *)
+
+  (* This lemma can of course be derived from the two above.
+      However, its proof itself is even simpler. *)
   Lemma opsem_reduce_seq3: forall hs1 s1 f1 es1 hs2 s2 f2 es2 vs es0,
       const_list vs ->
       reduce hs1 s1 f1 es1 hs2 s2 f2 es2 ->
       reduce hs1 s1 f1 (vs ++ es1 ++ es0) hs2 s2 f2 (vs ++ es2 ++ es0).
   Proof.
-  Admitted.
+(* REVISIT: prove this from scratch. *)
+    intros. rename H into Hvs. rename H0 into Hred.
+    apply opsem_reduce_seq2. apply Hvs.
+    apply opsem_reduce_seq1. apply Hred.
+(*! Uses admitted opsem_reduce_seq1 and opsem_reduce_seq2' !*)
+  Qed.
 
   
   
-
+(*** DEPRECATED
   (* Typing lemmas *)
 
   (* An easier one to get started *)
 
   
-  (* In properties.v, there's a proof of another verison of this lemma with the goal being the non-constructive exists. However, that proof relies on inverting the typing rule, which cannot be used here due to the goal being a sigma type (try coping the proof and see where it goes wrong; the tactic auto_prove_bet has to be copied here as well for that to be observed).
-     Find a way to prove this lemma with goal being the sigma-typed exists; likely it should be done by an induction on es1 or a destruct of e (or both). This might be quite difficult.
- *)
+  (* In properties.v, there's a proof of another verison of this lemma
+      with the goal being the non-constructive exists.
+      However, that proof relies on inverting the typing rule,
+      which cannot be used here due to the goal being a sigma type
+      (try coping the proof and see where it goes wrong;
+        the tactic auto_prove_bet has to be copied here as well for that to be observed).
+      Find a way to prove this lemma with goal being the sigma-typed exists;
+      likely it should be done by an induction on es1 or a destruct of e (or both).
+      This might be quite difficult. *)
   Lemma composition_typing_single_sig: forall C es1 e t1s t2s,
     be_typing C (es1 ++ [::e]) (Tf t1s t2s) ->
     { ts & { t1s' & { t2s' & { t3s | t1s = ts ++ t1s' /\
@@ -89,7 +272,8 @@ Section intro.
   Proof.
   Admitted.
 
-  (* Another composition typing lemma, with the second component being a general list instead of just a singleton. *)
+  (* Another composition typing lemma,
+      with the second component being a general list instead of just a singleton. *)
   Lemma composition_typing_sig: forall C es1 es2 t1s t2s,
       be_typing C (es1 ++ es2) (Tf t1s t2s) ->
       { ts & { t1s' & { t2s' & { t3s | t1s = ts ++ t1s' /\
@@ -98,7 +282,7 @@ Section intro.
                                          be_typing C es2 (Tf t3s t2s') }}}}.
   Proof.
   Admitted.
-  
+***)
 
 
   
@@ -106,28 +290,68 @@ Section intro.
   (* Here is a simple program that involves loops. Observe the code below. *)
   Definition i32_of_Z (z: Z) := VAL_int32 (Wasm_int.int_of_Z i32m z).
 
+  (* Loop Body (raw pseudocode):
+   *  stack.push(locals[0])
+   *  stack.push((testop (type: T_i32) (op: TO_eqz)) stack.pop())
+   *  if (stack.pop() == (i32) 0): stack.push(BI_br (label: 1))
+   *  stack.push(locals[0])
+   *  stack.push(locals[1])
+   *  stack.push((binop (type: T_i32) (op: Binop_i BOI_add)) stack.pop() stack.pop())
+   *  locals[1] = stack.pop()
+   *  stack.push(locals[0])
+   *  stack.push((i32) 1)
+   *  stack.push((binop (type: T_i32) (op: Binop_i BOI_sub)) stack.pop() stack.pop())
+   *  locals[0] = stack.pop()
+   *)
+  (* Loop Body (pseudocode):
+   *  Apply TO_eqz (=? 0) to locals[0] (if 0 then 1 else 0)
+   *    If this is non-zero, then break loop (i.e. break if locals[0] == 0)
+   *  Set locals[1] to the sum of locals[0] and locals[1]
+   *  Decrement locals[0]
+   *)
+
   Definition loop_body : seq basic_instruction :=
     [ :: BI_get_local 0; BI_testop T_i32 TO_eqz; BI_br_if 1;
       BI_get_local 0; BI_get_local 1; BI_binop T_i32 (Binop_i BOI_add); BI_set_local 1;
       BI_get_local 0; BI_const (i32_of_Z 1); BI_binop T_i32 (Binop_i BOI_sub); BI_set_local 0
     ].
   
+  (* Loop Body (raw pseudocode):
+   *  stack.push(label[block]) {ves split: ([stack.push(locals[0])], [])}
+   *  stack.push(label[loop]) {ves split: ([stack.push(locals[0])], [])}
+   *  (Loop Body)
+   *)
+  (* Loop Body (pseudocode):
+   *  Create a new scope with a while true loop of content: Loop Body
+   *  Exit when locals[0] is 0
+   *    On exit, locals[1] holds sum of all naturals upto the original locals[0]
+   *)
+  
   Definition code : seq administrative_instruction :=
     [:: AI_basic (BI_block (Tf [:: T_i32] [:: T_i32]) [:: BI_loop (Tf [:: T_i32] [:: T_i32]) loop_body ]);
      AI_basic (BI_get_local 1)].
 
-  Definition result_place_holder : seq administrative_instruction.
-  Admitted.
+  Definition result_place_holder : Z -> seq administrative_instruction :=
+    fun n => [:: AI_basic (BI_const (i32_of_Z ( (n*(n+1))/2 )))].
   
-  (* Try to work out what it does under the given premises, and fill in the above definition that specifies the execution result. Proving the reduction might be actually very tedious. *)
+  (* Try to work out what it does under the given premises,
+      and fill in the above definition that specifies the execution result.
+      Proving the reduction might be actually very tedious. *)
     Lemma opsem_reduce_loop: forall hs s f (z:Z),
       (z >= 0)%Z ->
       f.(f_locs) = [:: i32_of_Z z; i32_of_Z 0] ->
-      exists f', reduce_trans (hs, s, f, code) (hs, s, f', result_place_holder).
+      exists f', reduce_trans (hs, s, f, code) (hs, s, f', result_place_holder z).
   Proof.
+    intros. rename H into Hzpos. rename H0 into Hstore.
+  (*destruct f as [ff_locs ff_inst].
+    exists {|
+      f_locs := [:: i32_of_Z _; i32_of_Z 0];
+      f_inst := ff_inst
+    |}.*)
+    exists f. (* Same initialisation since equivalent code *)
+  (*unfold reduce_trans. unfold opsem.reduce_trans.*)
+  (*unfold result_place_holder. unfold code. unfold loop_body.*)
   Admitted.
   
 
 End intro.
-    
-
